ironfleet/src/Dafny/Distributed/Protocol/RSL/FailureProof/Failover2/FailureDetection_toplevel.i.dfy
@@ -7,79 +7,103 @@ include "FailureDetection_helper1.i.dfy"
 include "../Common/assumptions.i.dfy"
 
 include "../../CommonProof/Constants.i.dfy"
-module FailureDetection_i {
+include "FailureDetection.i.dfy"
+include "FailureDetection_final.i.dfy"
+
+module FailureDetection_toplevel_i {
 import opened TimestampedRslSystem_i
 import opened FailureHelpers_i
 import opened FailureDetection_defns_i
 import opened FailureDetection_helper0_i
 import opened FailureDetection_helper1_i
+import opened FailureDetection_i
 import opened Common_Assumptions
+import opened FailureDetection_final_i
 
-predicate FailoverFinal(s:TimestampedRslState)
+lemma InvariantsHoldInitially(s:TimestampedRslState)
+  requires FOAssumption(s)
+  requires exists con :: TimestampedRslInit(con, s)
+  ensures InView1(s, {})
+  ensures DelayInvs(s)
 {
-  && (forall pkt ::
-     pkt in s.t_environment.sentPackets ==>
 
-     && (pkt.msg.v.RslMessage_Heartbeat? ==>
-     pkt.msg.v.bal_heartbeat == Ballot(1, 0))
-     && (pkt.msg.v.RslMessage_2a? ==>
-     pkt.msg.v.bal_2a == Ballot(1, 0))
-     && (pkt.msg.v.RslMessage_2b? ==>
-     pkt.msg.v.bal_2b == Ballot(1, 0))
-     && (pkt.msg.v.RslMessage_1a? ==>
-     pkt.msg.v.bal_1a == Ballot(1, 0))
-     && (pkt.msg.v.RslMessage_1b? ==>
-     pkt.msg.v.bal_1b == Ballot(1, 0))
-  )
-
-  && s.t_replicas[1].v.replica.proposer.election_state.current_view == Ballot(1,1)
-  // FIXME: want to know that replicas[1] is in current_state == ??
-  && s.t_replicas[1].v.nextActionIndex == 9 // just checked for quorum of views, and got one
-  && TimeLe(s.t_replicas[1].ts, FailoverTime())
 }
 
-lemma FailoverTopLevel(tglb:seq<TimestampedRslState>) returns (startPhase1Idx:int)
-  requires exists con :: ValidTimestampedRSLBehavior(con, tglb)
-  // requires forall i | 0 <= i < |tglb| :: RslConsistency(tglb[i])
-  requires forall i | 0 <= i < |tglb| :: FOAssumption(tglb[i])
-  requires forall i | 0 <= i < |tglb| :: |tglb[i].t_replicas| > 2
-  // FIXME: also the 2-step assumptions have to be met
-
-  ensures forall j :: 0 <= j < |tglb| ==> j < startPhase1Idx ==>
-    var s := tglb[j];
-    && CurrView(s) // This means every node is in view (1,0); will rename to be more clear
-    && InView1Packets(s); // All packets have Ballot(1,0)
-
-  // The idx might be larger than the seq if the behavior given never has
-  // failover happen, and never reaches failover final
-  ensures startPhase1Idx >= 0
-  ensures startPhase1Idx < |tglb| ==> FailoverFinal(tglb[startPhase1Idx])
-
-  // TODO: Implement these post conditions
-  ensures forall i | 0 <= i < |tglb| :: 
-    forall pkt | pkt in tglb[i].t_environment.sentPackets :: !IsNewReplyPacket(tglb[i], pkt)
+predicate FailoverInv(s:TimestampedRslState)
+  requires CommonAssumptions(s)
 {
-  // TODO:
-  assume false;
+  (DelayInvs(s) &&
+    (exists sr :: InView1(s, sr))) || FinalStage(s)
 }
 
+lemma FailoverInvMaintained(s:TimestampedRslState, s':TimestampedRslState)
+  requires CommonAssumptions(s) && CommonAssumptions(s');
+  requires FOAssumption2State(s,s')
+  requires InFailover(s);
+  requires InFailover(s) ==> FOAssumption(s);
+  requires InFailover(s') ==> FOAssumption(s');
+  requires TimestampedRslNext(s, s');
+  requires FailoverInv(s);
+
+  ensures InFailover(s') || InPhase1(s');
+  ensures InFailover(s') ==> FailoverInv(s');
+  ensures InPhase1(s') ==> FailoverFinal(s');
+{
+  if FinalStage(s) {
+    FinalStageInd(s, s');
+    if FailoverFinal(s') {
+      assert InPhase1(s');
+      assert FailoverFinal(s');
+      return;
+    } else {
+      assert InFailover(s');
+      assert FinalStage(s');
+      return;
+    }
+  } else {
+    var sr :| InView1(s, sr);
+    assert InFailover(s');
+    assert FOAssumption(s');
+    var sr' := InView1_ind(s, s', sr);
+    DelayInv_ind(s, s');
+    assert FailoverInv(s');
+  }
+}
+/*
 lemma FailoverTopLevel_Prototype(tglb:seq<TimestampedRslState>) returns (startPhase1Idx:int)
   requires exists con :: ValidTimestampedRSLBehavior(con, tglb)
   requires InFailover(tglb[0])
-  requires forall i | 0 <= i < |tglb| :: InFailover(tglb[i]) ==> FOAssumption(tglb[i])
-  requires forall i | 0 <= i < |tglb| :: |tglb[i].t_replicas| > 2
-  ensures forall j :: 0 <= j < |tglb| ==> j < startPhase1Idx ==>
-    var s := tglb[j];
-    && CurrView(s) // This means every node is in view (1,0); will rename to be more clear
-    && InView1Packets(s); // All packets have Ballot(1,0)
-  ensures startPhase1Idx >= 0
-  ensures startPhase1Idx < |tglb| ==> FailoverFinal(tglb[startPhase1Idx])
-  ensures startPhase1Idx < |tglb| ==> InPhase1(tglb[startPhase1Idx])
-  ensures forall i | 0 <= i < |tglb| ::
-    forall pkt | pkt in tglb[i].t_environment.sentPackets :: !IsNewReplyPacket(tglb[i], pkt)
-{
-  // TODO:
-  assume false;
-}
+  requires forall i :: 0 <= i < |tglb| ==> InFailover(tglb[i]) ==> FOAssumption(tglb[i])
+  requires forall i :: 0 <= i < |tglb| ==> |tglb[i].t_replicas| > 2
 
+  // ensures startPhase1Idx >= 0
+  // ensures startPhase1Idx < |tglb| ==> FailoverFinal(tglb[startPhase1Idx])
+  // ensures startPhase1Idx < |tglb| ==> InPhase1(tglb[startPhase1Idx])
+  // ensures forall i | 0 <= i < |tglb| ::
+    // forall pkt | pkt in tglb[i].t_environment.sentPackets :: !IsNewReplyPacket(tglb[i], pkt)
+{
+  startPhase1Idx := 0;
+
+  var i := 1;
+  InvariantsHoldInitially(tglb[0]);
+
+  assert FailoverInv(tglb[0]);
+  while i < |tglb|
+    invariant i > 0
+    invariant i <= |tglb|
+    invariant FailoverInv(tglb[i - 1])
+    invariant InFailover(tglb[i - 1])
+  {
+    var s := tglb[i-1];
+    var s' := tglb[i];
+    var sr :| InView1(s, sr);
+    var sr' := InView1_ind(s, s', sr);
+    if FinalStage(s') {
+      return i;
+    } else {
+      i := i + 1;
+    }
+  }
+}
+*/
 }
